Foundation/FirstOrder/Kripke/WeakForcing.lean
@@ -6,34 +6,39 @@ import Foundation.FirstOrder.NegationTranslation.GoedelGentzen
 Main reference: Jeremy Avigad, "Forcing in proof theory"
 -/
 
-namespace LO.FirstOrder.KripkeModel
+namespace LO.FirstOrder
 
-variable {L : Language} [L.Relational] {ℙ : KripkeModel L}
+variable {L : Language} [L.Relational]
 
-def WeaklyForces (p : ℙ) (bv : Fin n → ℙ.Name) (fv : ξ → ℙ.Name) (φ : Semiformula L ξ n) : Prop := ℙ.Forces p bv fv φᴺ
+namespace KripkeModel
 
-local notation:45 p " ⊩[" bv "|" fv "] " φ:46 => WeaklyForces p bv fv φ
+variable {ℙ : Type*} [Preorder ℙ] {Name : Type*} [KripkeModel L ℙ Name]
+
+def WeaklyForces (p : ℙ) (bv : Fin n → Name) (fv : ξ → Name) (φ : Semiformula L ξ n) : Prop := Forces p bv fv φᴺ
+
+scoped notation:45 p " ⊩ᶜ[" bv "|" fv "] " φ:46 => WeaklyForces p bv fv φ
 
 @[simp] lemma exists_le {α : Type*} [Preorder α] (a : α) : ∃ x, x ≤ a := ⟨a, by rfl⟩
+
 namespace WeaklyForces
 
-variable {bv : Fin n → ℙ.Name} {fv : ξ → ℙ.Name}
+variable {p q r : ℙ} {bv : Fin n → Name} {fv : ξ → Name}
 
 @[simp] lemma rel {R : L.Rel k} {t : Fin k → Semiterm L ξ n} :
-    p ⊩[bv|fv] Semiformula.rel R t ↔ ∀ q ≤ p, ∃ r ≤ q, ℙ.Rel r R fun i ↦ (t i).relationalVal bv fv := by simp [WeaklyForces]
+    p ⊩ᶜ[bv|fv] Semiformula.rel R t ↔ ∀ q ≤ p, ∃ r ≤ q, Rel r R fun i ↦ (t i).relationalVal bv fv := by simp [WeaklyForces]
 
 @[simp] lemma nrel {R : L.Rel k} {t : Fin k → Semiterm L ξ n} :
-    p ⊩[bv|fv] Semiformula.nrel R t ↔ ∀ q ≤ p, ¬ℙ.Rel q R fun i ↦ (t i).relationalVal bv fv := by simp [WeaklyForces]
+    p ⊩ᶜ[bv|fv] Semiformula.nrel R t ↔ ∀ q ≤ p, ¬Rel q R fun i ↦ (t i).relationalVal bv fv := by simp [WeaklyForces]
 
-@[simp] lemma verum : p ⊩[bv|fv] (⊤ : Semiformula L ξ n) := by simp [WeaklyForces]
+@[simp] lemma verum : p ⊩ᶜ[bv|fv] (⊤ : Semiformula L ξ n) := by simp [WeaklyForces]
 
-@[simp] lemma falsum : ¬p ⊩[bv|fv] (⊥ : Semiformula L ξ n) := by rintro ⟨⟩
+@[simp] lemma falsum : ¬p ⊩ᶜ[bv|fv] (⊥ : Semiformula L ξ n) := by rintro ⟨⟩
 
 @[simp] lemma and {φ ψ : Semiformula L ξ n} :
-    p ⊩[bv|fv] φ ⋏ ψ ↔ p ⊩[bv|fv] φ ∧ p ⊩[bv|fv] ψ := by simp [WeaklyForces]
+    p ⊩ᶜ[bv|fv] φ ⋏ ψ ↔ p ⊩ᶜ[bv|fv] φ ∧ p ⊩ᶜ[bv|fv] ψ := by simp [WeaklyForces]
 
 @[simp] lemma or {φ ψ : Semiformula L ξ n} :
-    p ⊩[bv|fv] φ ⋎ ψ ↔ ∀ q ≤ p, ∃ r ≤ q, r ⊩[bv|fv] φ ∨ r ⊩[bv|fv] ψ := by
+    p ⊩ᶜ[bv|fv] φ ⋎ ψ ↔ ∀ q ≤ p, ∃ r ≤ q, r ⊩ᶜ[bv|fv] φ ∨ r ⊩ᶜ[bv|fv] ψ := by
   suffices
       (∀ q ≤ p, (∃ r ≤ q, Forces r bv fv φᴺ) ∨ ∃ r ≤ q, Forces r bv fv ψᴺ) ↔
       ∀ q ≤ p, ∃ r ≤ q, Forces r bv fv φᴺ ∨ Forces r bv fv ψᴺ by
@@ -41,106 +46,106 @@ variable {bv : Fin n → ℙ.Name} {fv : ξ → ℙ.Name}
   grind
 
 @[simp] lemma all {φ : Semiformula L ξ (n + 1)} :
-    p ⊩[bv|fv] ∀' φ ↔ ∀ q ≤ p, ∀ x : q, WeaklyForces q (x :> bv) fv φ := by simp [WeaklyForces]
+    p ⊩ᶜ[bv|fv] ∀' φ ↔ ∀ q ≤ p, ∀ x : q, WeaklyForces q (↑x :> bv) fv φ := by simp [WeaklyForces]
 
 @[simp] lemma ex {φ : Semiformula L ξ (n + 1)} :
-    p ⊩[bv|fv] ∃' φ ↔ ∀ q ≤ p, ∃ r ≤ q, ∃ x : r, r ⊩[x :> bv|fv] φ := by
+    p ⊩ᶜ[bv|fv] ∃' φ ↔ ∀ q ≤ p, ∃ r ≤ q, ∃ x : r, r ⊩ᶜ[↑x :> bv|fv] φ := by
   suffices
-      (∀ q ≤ p, ∃ r ≤ q, ∃ x ∈ ℙ.Domain r, ∃ s ≤ r, s ⊩[x :> bv|fv] φ) ↔
-      (∀ q ≤ p, ∃ r ≤ q, ∃ x ∈ ℙ.Domain r, r ⊩[x :> bv|fv] φ) by
+      (∀ q ≤ p, ∃ r ≤ q, ∃ x ∈ Domain r, ∃ s ≤ r, s ⊩ᶜ[x :> bv|fv] φ) ↔
+      (∀ q ≤ p, ∃ r ≤ q, ∃ x ∈ Domain r, r ⊩ᶜ[x :> bv|fv] φ) by
     simpa [WeaklyForces]
   constructor
   · intro h q hqp
     rcases h q hqp with ⟨r, hrq, x, hx, s, hsr, H⟩
-    exact ⟨s, le_trans hsr hrq, x, ℙ.domain_antimonotone hsr hx, H⟩
+    exact ⟨s, le_trans hsr hrq, x, domain_antimonotone hsr hx, H⟩
   · intro h q hqp
     rcases h q hqp with ⟨r, hrq, x, hx, H⟩
     exact ⟨r, hrq, x, hx, r, by rfl, H⟩
 
 lemma monotone {φ : Semiformula L ξ n} :
-    p ⊩[bv|fv] φ → ∀ q ≤ p, q ⊩[bv|fv] φ := fun h ↦ Forces.monotone h
+    p ⊩ᶜ[bv|fv] φ → ∀ q ≤ p, q ⊩ᶜ[bv|fv] φ := fun h ↦ Forces.monotone h
 
-lemma genricity {n} {bv : Fin n → ℙ.Name} {fv : ξ → ℙ.Name} {φ : Semiformula L ξ n} :
-    (∀ q ≤ p, ∃ r ≤ q, r ⊩[bv|fv] φ) → p ⊩[bv|fv] φ :=
+lemma generic {p : ℙ} {n} {bv : Fin n → Name} {fv : ξ → Name} {φ : Semiformula L ξ n} :
+    (∀ q ≤ p, ∃ r ≤ q, r ⊩ᶜ[bv|fv] φ) → p ⊩ᶜ[bv|fv] φ :=
   match φ with
   | .rel R v => by
     suffices
-      (∀ q ≤ p, ∃ r ≤ q, ∀ q ≤ r, ∃ s ≤ q, ℙ.Rel s R fun i ↦ (v i).relationalVal bv fv) →
-      (∀ q ≤ p, ∃ r ≤ q, ℙ.Rel r R fun i ↦ (v i).relationalVal bv fv) by simpa
+      (∀ q ≤ p, ∃ r ≤ q, ∀ q ≤ r, ∃ s ≤ q, Rel s R fun i ↦ (v i).relationalVal bv fv) →
+      (∀ q ≤ p, ∃ r ≤ q, Rel r R fun i ↦ (v i).relationalVal bv fv) by simpa
     intro h q hqp
     rcases h q hqp with ⟨r, hrq, H⟩
     rcases H r (by rfl) with ⟨s, hsr, Hs⟩
     exact ⟨s, le_trans hsr hrq, Hs⟩
   | .nrel R v => by
     suffices
-      (∀ q ≤ p, ∃ r ≤ q, ∀ s ≤ r, ¬ℙ.Rel s R fun i ↦ (v i).relationalVal bv fv) →
-      (∀ q ≤ p, ¬ℙ.Rel q R fun i ↦ (v i).relationalVal bv fv) by simpa
+      (∀ q ≤ p, ∃ r ≤ q, ∀ s ≤ r, ¬Rel s R fun i ↦ (v i).relationalVal bv fv) →
+      (∀ q ≤ p, ¬Rel q R fun i ↦ (v i).relationalVal bv fv) by simpa
     intro h q hqp hR
     rcases h q hqp with ⟨r, hrq, Hr⟩
-    exact Hr r (by rfl) (ℙ.rel_monotone hR r hrq)
+    exact Hr r (by rfl) (rel_monotone hR r hrq)
   | ⊤ => by simp
   | ⊥ => by simp
   | φ ⋏ ψ => by
-    suffices (∀ q ≤ p, ∃ r ≤ q, r ⊩[bv|fv] φ ∧ r ⊩[bv|fv] ψ) → p ⊩[bv|fv] φ ∧ p ⊩[bv|fv] ψ by simpa
+    suffices (∀ q ≤ p, ∃ r ≤ q, r ⊩ᶜ[bv|fv] φ ∧ r ⊩ᶜ[bv|fv] ψ) → p ⊩ᶜ[bv|fv] φ ∧ p ⊩ᶜ[bv|fv] ψ by simpa
     intro h
-    refine ⟨genricity fun q hqp ↦ ?_, genricity fun q hqp ↦ ?_⟩
+    refine ⟨generic fun q hqp ↦ ?_, generic fun q hqp ↦ ?_⟩
     · rcases h q hqp with ⟨r, hrq, h, _⟩
       exact ⟨r, hrq, h⟩
     · rcases h q hqp with ⟨r, hrq, _, h⟩
       exact ⟨r, hrq, h⟩
   | φ ⋎ ψ => by
     suffices
-      (∀ q ≤ p, ∃ r ≤ q, ∀ q ≤ r, ∃ r ≤ q, r ⊩[bv|fv] φ ∨ r ⊩[bv|fv] ψ) →
-      (∀ q ≤ p, ∃ r ≤ q, r ⊩[bv|fv] φ ∨ r ⊩[bv|fv] ψ) by simpa
+      (∀ q ≤ p, ∃ r ≤ q, ∀ q ≤ r, ∃ r ≤ q, r ⊩ᶜ[bv|fv] φ ∨ r ⊩ᶜ[bv|fv] ψ) →
+      (∀ q ≤ p, ∃ r ≤ q, r ⊩ᶜ[bv|fv] φ ∨ r ⊩ᶜ[bv|fv] ψ) by simpa
     intro h q hqp
     rcases h q hqp with ⟨r, hrq, H⟩
     rcases H r (by rfl) with ⟨s, hsr, Hs⟩
     exact ⟨s, le_trans hsr hrq, Hs⟩
   | ∀' φ => by
     suffices
-      (∀ q ≤ p, ∃ r ≤ q, ∀ q ≤ r, ∀ a ∈ ℙ.Domain q, q ⊩[a :> bv|fv] φ) →
-      (∀ q ≤ p, ∀ x ∈ ℙ.Domain q, q ⊩[x :> bv|fv] φ) by simpa
+      (∀ q ≤ p, ∃ r ≤ q, ∀ q ≤ r, ∀ a ∈ Domain q, q ⊩ᶜ[a :> bv|fv] φ) →
+      (∀ q ≤ p, ∀ x ∈ Domain q, q ⊩ᶜ[x :> bv|fv] φ) by simpa
     intro h q hqp x hx
-    apply genricity
+    apply generic
     intro r hrq
     rcases h r (le_trans hrq hqp) with ⟨s, hsr, Hs⟩
-    exact ⟨s, hsr, Hs s (by rfl) x (ℙ.domain_antimonotone' hx _ (le_trans hsr hrq))⟩
+    exact ⟨s, hsr, Hs s (by rfl) x (domain_monotone hx _ (le_trans hsr hrq))⟩
   | ∃' φ => by
     suffices
-      (∀ q ≤ p, ∃ r ≤ q, ∀ q ≤ r, ∃ r ≤ q, ∃ x ∈ ℙ.Domain r, r ⊩[x :> bv|fv] φ) →
-      (∀ q ≤ p, ∃ r ≤ q, ∃ x ∈ ℙ.Domain r, r ⊩[x :> bv|fv] φ) by simpa
+      (∀ q ≤ p, ∃ r ≤ q, ∀ q ≤ r, ∃ r ≤ q, ∃ x ∈ Domain r, r ⊩ᶜ[x :> bv|fv] φ) →
+      (∀ q ≤ p, ∃ r ≤ q, ∃ x ∈ Domain r, r ⊩ᶜ[x :> bv|fv] φ) by simpa
     intro h q hqp
     rcases h q hqp with ⟨r, hrq, H⟩
     rcases H r (by rfl) with ⟨s, hsr, x, hx, H⟩
     exact ⟨s, le_trans hsr hrq, x, hx, H⟩
 
-lemma genricity_iff {φ : Semiformula L ξ n} :
-    p ⊩[bv|fv] φ ↔ ∀ q ≤ p, ∃ r ≤ q, r ⊩[bv|fv] φ :=
-  ⟨fun H q hqp ↦ ⟨q, by rfl, H.monotone q hqp⟩, genricity⟩
+lemma generic_iff {φ : Semiformula L ξ n} :
+    p ⊩ᶜ[bv|fv] φ ↔ ∀ q ≤ p, ∃ r ≤ q, r ⊩ᶜ[bv|fv] φ :=
+  ⟨fun H q hqp ↦ ⟨q, by rfl, H.monotone q hqp⟩, generic⟩
 
-lemma genricity_iff_not {φ : Semiformula L ξ n} :
-    ¬p ⊩[bv|fv] φ ↔ ∃ q ≤ p, ∀ r ≤ q, ¬r ⊩[bv|fv] φ := by simpa using genricity_iff.not
+lemma generic_iff_not {φ : Semiformula L ξ n} :
+    ¬p ⊩ᶜ[bv|fv] φ ↔ ∃ q ≤ p, ∀ r ≤ q, ¬r ⊩ᶜ[bv|fv] φ := by simpa using generic_iff.not
 
-@[simp] lemma not {n} {bv : Fin n → ℙ.Name} {fv : ξ → ℙ.Name} {φ : Semiformula L ξ n} :
-    p ⊩[bv|fv] ∼φ ↔ ∀ q ≤ p, ¬q ⊩[bv|fv] φ :=
+@[simp] lemma not {p : ℙ} {n} {bv : Fin n → Name} {fv : ξ → Name} {φ : Semiformula L ξ n} :
+    p ⊩ᶜ[bv|fv] ∼φ ↔ ∀ q ≤ p, ¬q ⊩ᶜ[bv|fv] φ :=
   match φ with
   | .rel R v => by
     suffices
-      (∀ q ≤ p, ¬ℙ.Rel q R fun i ↦ (v i).relationalVal bv fv) ↔
-      (∀ q ≤ p, ∃ r ≤ q, ∀ s ≤ r, ¬ℙ.Rel s R fun i ↦ (v i).relationalVal bv fv) by simpa
+      (∀ q ≤ p, ¬Rel q R fun i ↦ (v i).relationalVal bv fv) ↔
+      (∀ q ≤ p, ∃ r ≤ q, ∀ s ≤ r, ¬Rel s R fun i ↦ (v i).relationalVal bv fv) by simpa
     constructor
     · intro h q hqp
       exact ⟨q, by rfl, fun r hrq ↦ h r (le_trans hrq hqp)⟩
     · intro h q hqp H
       rcases h q hqp with ⟨r, hrq, Hr⟩
-      exact Hr r (by rfl) (ℙ.rel_monotone H _ hrq)
+      exact Hr r (by rfl) (rel_monotone H _ hrq)
   | .nrel R v => by simp
   | ⊤ => by simp
   | ⊥ => by simp
   | φ ⋏ ψ => by
     suffices
-        (∀ q ≤ p, ∃ r ≤ q, r ⊩[bv|fv] ∼φ ∨ r ⊩[bv|fv] ∼ψ) ↔
-        (∀ q ≤ p, ¬q ⊩[bv|fv] φ ∨ ¬q ⊩[bv|fv] ψ) by
+        (∀ q ≤ p, ∃ r ≤ q, r ⊩ᶜ[bv|fv] ∼φ ∨ r ⊩ᶜ[bv|fv] ∼ψ) ↔
+        (∀ q ≤ p, ¬q ⊩ᶜ[bv|fv] φ ∨ ¬q ⊩ᶜ[bv|fv] ψ) by
       simpa [-not_and, not_and_or]
     constructor
     · intro h q hqp
@@ -151,16 +156,16 @@ lemma genricity_iff_not {φ : Semiformula L ξ n} :
         exact WeaklyForces.not.mp H r (by rfl) (Hqψ.monotone _ hrq)
     · intro h q hqp
       rcases h q hqp with (C | C)
-      · rcases genricity_iff_not.mp C with ⟨r, hrq, Hr⟩
+      · rcases generic_iff_not.mp C with ⟨r, hrq, Hr⟩
         refine ⟨r, hrq, ?_⟩
         left; apply WeaklyForces.not.mpr Hr
-      · rcases genricity_iff_not.mp C with ⟨r, hrq, Hr⟩
+      · rcases generic_iff_not.mp C with ⟨r, hrq, Hr⟩
         refine ⟨r, hrq, ?_⟩
         right; apply WeaklyForces.not.mpr Hr
   | φ ⋎ ψ => by
     suffices
-      p ⊩[bv|fv] ∼φ ∧ p ⊩[bv|fv] ∼ψ ↔
-      ∀ q ≤ p, ∃ r ≤ q, ∀ s ≤ r, ¬s ⊩[bv|fv] φ ∧ ¬s ⊩[bv|fv] ψ by simpa
+      p ⊩ᶜ[bv|fv] ∼φ ∧ p ⊩ᶜ[bv|fv] ∼ψ ↔
+      ∀ q ≤ p, ∃ r ≤ q, ∀ s ≤ r, ¬s ⊩ᶜ[bv|fv] φ ∧ ¬s ⊩ᶜ[bv|fv] ψ by simpa
     constructor
     · intro h q hqp
       refine ⟨q, by rfl, fun r hrq ↦ ⟨?_, ?_⟩⟩
@@ -178,20 +183,20 @@ lemma genricity_iff_not {φ : Semiformula L ξ n} :
         exact (H r (by rfl)).2 (Hq.monotone _ hrq)
   | ∀' φ => by
     suffices
-      (∀ q ≤ p, ∃ r ≤ q, ∃ a ∈ ℙ.Domain r, r ⊩[a :> bv|fv] ∼φ) ↔
-      (∀ q ≤ p, ∃ r ≤ q, ∃ x ∈ ℙ.Domain r, ¬r ⊩[x :> bv|fv] φ) by simpa
+      (∀ q ≤ p, ∃ r ≤ q, ∃ a ∈ Domain r, r ⊩ᶜ[a :> bv|fv] ∼φ) ↔
+      (∀ q ≤ p, ∃ r ≤ q, ∃ x ∈ Domain r, ¬r ⊩ᶜ[x :> bv|fv] φ) by simpa
     constructor
     · intro h q hqp
       rcases h q hqp with ⟨r, hrq, x, hx, Hr⟩
       exact ⟨r, hrq, x, hx, WeaklyForces.not.mp Hr r (by rfl)⟩
     · intro h q hqp
       rcases h q hqp with ⟨r, hrq, x, hx, H⟩
-      rcases genricity_iff_not.mp H with ⟨s, hsr, Hs⟩
-      exact ⟨s, le_trans hsr hrq, x, ℙ.domain_antimonotone hsr hx, WeaklyForces.not.mpr Hs⟩
+      rcases generic_iff_not.mp H with ⟨s, hsr, Hs⟩
+      exact ⟨s, le_trans hsr hrq, x, domain_antimonotone hsr hx, WeaklyForces.not.mpr Hs⟩
   | ∃' φ => by
     suffices
-      (∀ q ≤ p, ∀ a ∈ ℙ.Domain q, q ⊩[a :> bv|fv] ∼φ) ↔
-      (∀ q ≤ p, ∃ r ≤ q, ∀ s ≤ r, ∀ x ∈ ℙ.Domain s, ¬s ⊩[x :> bv|fv] φ) by simpa
+      (∀ q ≤ p, ∀ a ∈ Domain q, q ⊩ᶜ[a :> bv|fv] ∼φ) ↔
+      (∀ q ≤ p, ∃ r ≤ q, ∀ s ≤ r, ∀ x ∈ Domain s, ¬s ⊩ᶜ[x :> bv|fv] φ) by simpa
     constructor
     · intro h q hqp
       refine ⟨q, by rfl, ?_⟩
@@ -201,42 +206,42 @@ lemma genricity_iff_not {φ : Semiformula L ξ n} :
       apply WeaklyForces.not.mpr
       intro r hrq Hr
       rcases h r (le_trans hrq hqp) with ⟨s, hsr, H⟩
-      have : ¬s ⊩[x :> bv|fv] φ := H s (by rfl) x (ℙ.domain_antimonotone (le_trans hsr hrq) hx)
+      have : ¬s ⊩ᶜ[x :> bv|fv] φ := H s (by rfl) x (domain_antimonotone (le_trans hsr hrq) hx)
       exact this (Hr.monotone _ hsr)
 
-lemma genricity_iff_not' {φ : Semiformula L ξ n} :
-    ¬p ⊩[bv|fv] φ ↔ ∃ q ≤ p, q ⊩[bv|fv] ∼φ := by simpa using genricity_iff.not
+lemma generic_iff_not' {φ : Semiformula L ξ n} :
+    ¬p ⊩ᶜ[bv|fv] φ ↔ ∃ q ≤ p, q ⊩ᶜ[bv|fv] ∼φ := by simpa using generic_iff.not
 
 @[simp] lemma imply {φ ψ : Semiformula L ξ n} :
-    p ⊩[bv|fv] φ ➝ ψ ↔ ∀ q ≤ p, q ⊩[bv|fv] φ → q ⊩[bv|fv] ψ := by
+    p ⊩ᶜ[bv|fv] φ ➝ ψ ↔ ∀ q ≤ p, q ⊩ᶜ[bv|fv] φ → q ⊩ᶜ[bv|fv] ψ := by
   suffices
-    (∀ q ≤ p, ∃ r ≤ q, (∀ q ≤ r, ¬q ⊩[bv|fv] φ) ∨ r ⊩[bv|fv] ψ) ↔
-    (∀ q ≤ p, q ⊩[bv|fv] φ → q ⊩[bv|fv] ψ) by simpa [DeMorgan.imply]
+    (∀ q ≤ p, ∃ r ≤ q, (∀ q ≤ r, ¬q ⊩ᶜ[bv|fv] φ) ∨ r ⊩ᶜ[bv|fv] ψ) ↔
+    (∀ q ≤ p, q ⊩ᶜ[bv|fv] φ → q ⊩ᶜ[bv|fv] ψ) by simpa [DeMorgan.imply]
   constructor
   · intro h q hqp Hqφ
     by_contra! Hqψ
-    rcases genricity_iff_not.mp Hqψ with ⟨r, hrq, Hr⟩
+    rcases generic_iff_not.mp Hqψ with ⟨r, hrq, Hr⟩
     rcases h r (le_trans hrq hqp) with ⟨s, hsr, (H | H)⟩
     · exact H s (by rfl) (Hqφ.monotone s (le_trans hsr hrq))
     · exact Hr s hsr H
   · intro h q hqp
-    have : ¬q ⊩[bv|fv] φ ∨ q ⊩[bv|fv] ψ := not_or_of_imp (h q hqp)
+    have : ¬q ⊩ᶜ[bv|fv] φ ∨ q ⊩ᶜ[bv|fv] ψ := not_or_of_imp (h q hqp)
     rcases this with (H | H)
-    · rcases genricity_iff_not.mp H with ⟨r, hrq, H⟩
+    · rcases generic_iff_not.mp H with ⟨r, hrq, H⟩
       exact ⟨r, hrq, Or.inl H⟩
     · exact ⟨q, by rfl, Or.inr H⟩
 
 @[simp] lemma iff {φ ψ : Semiformula L ξ n} :
-    p ⊩[bv|fv] φ ⭤ ψ ↔ ∀ q ≤ p, q ⊩[bv|fv] φ ↔ q ⊩[bv|fv] ψ := by
+    p ⊩ᶜ[bv|fv] φ ⭤ ψ ↔ ∀ q ≤ p, q ⊩ᶜ[bv|fv] φ ↔ q ⊩ᶜ[bv|fv] ψ := by
   simp [LogicalConnective.iff]; grind
 
 end WeaklyForces
 
-abbrev WeaklyForces₀ (p : ℙ) (φ : Sentence L) : Prop := p ⊩[![]|Empty.elim] ↑φ
+abbrev WeaklyForces₀ (p : ℙ) (φ : Sentence L) : Prop := p ⊩ᶜ[![]|Empty.elim] ↑φ
 
 instance : WeakForcingRelation ℙ (Sentence L) := ⟨WeaklyForces₀⟩
 
-lemma weaklyForces₀_def {p : ℙ} {φ : Sentence L} : p ⊩ᶜ φ ↔ p ⊩[![]|Empty.elim] φ := by rfl
+lemma weaklyForces₀_def {p : ℙ} {φ : Sentence L} : p ⊩ᶜ φ ↔ p ⊩ᶜ[![]|Empty.elim] φ := by rfl
 
 lemma weaklyForces₀_iff_forces {p : ℙ} {φ : Sentence L} :
     p ⊩ᶜ φ ↔ p ⊩ φᴺ := by rfl
@@ -245,20 +250,63 @@ namespace WeaklyForces₀
 
 lemma monotone {p : ℙ} : p ⊩ᶜ φ → ∀ q ≤ p, q ⊩ᶜ φ := WeaklyForces.monotone
 
-lemma genericity {p : ℙ} :
-    (∀ q ≤ p, ∃ r ≤ q, r ⊩ᶜ φ) → p ⊩ᶜ φ := WeaklyForces.genricity
+lemma generic {p : ℙ} :
+    (∀ q ≤ p, ∃ r ≤ q, r ⊩ᶜ φ) → p ⊩ᶜ φ := WeaklyForces.generic
 
-lemma genericity_iff {p : ℙ} :
-    p ⊩ᶜ φ ↔ ∀ q ≤ p, ∃ r ≤ q, r ⊩ᶜ φ := WeaklyForces.genricity_iff
+lemma generic_iff {p : ℙ} :
+    p ⊩ᶜ φ ↔ ∀ q ≤ p, ∃ r ≤ q, r ⊩ᶜ φ := WeaklyForces.generic_iff
 
 instance : WeakForcingRelation.ClassicalKripke ℙ (· ≥ ·) where
   verum w := by simp [weaklyForces₀_def]
-  falsum w := by simp [weaklyForces₀_def, WeakForcingRelation.NotForces]
+  falsum w := by simp [weaklyForces₀_def]
   and w := by simp [weaklyForces₀_def]
   or w := by simp [weaklyForces₀_def]
   imply w := by simp [weaklyForces₀_def]
-  not w := by simp [weaklyForces₀_def, WeakForcingRelation.NotForces]
+  not w := by simp [weaklyForces₀_def]
+  monotone := monotone
+  generic := generic
+
+lemma sound {T : Theory L} (b : T ⊢ φ) : ℙ ∀⊩ᶜ* T → ℙ ∀⊩ᶜ φ := fun H ↦
+  Forces₀.sound (W := ℙ) (gödel_gentzen b (Λ := 𝗜𝗻𝘁¹)) fun φ hφ ↦ (by
+    rcases show ∃ ψ ∈ T, ψᴺ = φ by simpa [Theory.ToTheoryᵢ] using hφ with ⟨ψ, hψ, rfl⟩
+    exact H ψ hψ)
 
 end WeaklyForces₀
 
 end KripkeModel
+
+/-- Kripke model for classical first-order logic -/
+def ForcingNotion (L : Language) [L.Relational] := IntKripke L
+
+namespace ForcingNotion
+
+variable (ℙ : ForcingNotion L)
+
+abbrev Condition := ℙ.World
+
+abbrev Name := ℙ.Carrier
+
+instance : CoeSort (ForcingNotion L) (Type _) := ⟨fun ℙ ↦ ℙ.Condition⟩
+
+instance : CoeSort ℙ (Type _) := ⟨fun p ↦ ℙ.Domain p⟩
+
+instance : Nonempty ℙ := ℙ.nonempty
+
+instance : Preorder ℙ := ℙ.preorder
+
+instance kripke : KripkeModel L ℙ ℙ.Name := IntKripke.kripke ℙ
+
+variable {ℙ}
+
+open KripkeModel
+
+instance : Semantics (ForcingNotion L) (Sentence L) := ⟨fun ℙ φ ↦ ℙ ∀⊩ᶜ φ⟩
+
+lemma models_def : ℙ ⊧ φ ↔ ℙ ∀⊩ᶜ φ := by rfl
+
+lemma sound {T : Theory L} (b : T ⊢ φ) : ℙ ⊧* T → ℙ ⊧ φ := fun H ↦
+  WeaklyForces₀.sound (ℙ := ℙ) b fun _ hφ ↦ H.models_set hφ
+
+instance (T : Theory L) : Sound T (Semantics.models (ForcingNotion L) T) := ⟨fun b _ H ↦ sound b H⟩
+
+end ForcingNotion
