Foundation/FirstOrder/NegationTranslation/GoedelGentzen.lean
@@ -1,4 +1,5 @@
 import Foundation.FirstOrder.Intuitionistic.Deduction
+import Foundation.Meta.IntProver
 
 namespace LO.FirstOrder
 
@@ -21,7 +22,7 @@ namespace Semiformula
 def doubleNegation {n} : Semiformula L ξ n → Semiformulaᵢ L ξ n
   | rel r v  => ∼∼(.rel r v)
   | nrel r v => ∼(.rel r v)
-  | ⊤        => ∼⊥
+  | ⊤        => ⊤
   | ⊥        => ⊥
   | φ ⋏ ψ    => φ.doubleNegation ⋏ ψ.doubleNegation
   | φ ⋎ ψ    => ∼(∼φ.doubleNegation ⋏ ∼ψ.doubleNegation)
@@ -46,8 +47,20 @@ scoped[LO.FirstOrder] postfix:max "ᴺ" => Semiformula.doubleNegation
 
 @[simp] lemma doubleNegation_ex (φ : Semiformula L ξ (n + 1)) : (∃' φ)ᴺ = ∼(∀' ∼φᴺ) := rfl
 
+lemma doubleNegation_imply (φ ψ : Semiformula L ξ n) : (φ ➝ ψ)ᴺ = ∼(∼(∼φ)ᴺ ⋏ ∼ψᴺ) := by simp [imp_eq]
+
 @[simp] lemma doubleNegation_isNegative (φ : Semiformula L ξ n) : φᴺ.IsNegative := by
   induction φ using rec' <;> simp [*]
+
+@[simp] lemma doubleNegation_conj₂ (Γ : List (Semiformula L ξ n)) :
+    (Γ.conj₂)ᴺ = (Γ.map Semiformula.doubleNegation).conj₂ :=
+  match Γ with
+  |          [] => by simp; rfl
+  |         [φ] => by simp
+  | φ :: ψ :: Γ => by simp [doubleNegation_conj₂ (ψ :: Γ)]
+
+lemma doubleNegation_fconj (s : Finset (Semiformula L ξ n)) :
+    (s.conj)ᴺ = (s.toList.map Semiformula.doubleNegation).conj₂ := doubleNegation_conj₂ _
 
 lemma rew_doubleNegation (ω : Rew L ξ₁ n₁ ξ₂ n₂) (φ : Semiformula L ξ₁ n₁) : ω ▹ φᴺ = (ω ▹ φ)ᴺ := by
   induction φ using rec' generalizing n₂ <;> simp [rew_rel, rew_nrel, Semiformulaᵢ.rew_rel, *]
@@ -60,99 +73,140 @@ lemma emb_doubleNegation (φ : Semisentence L n₁) :
 
 end Semiformula
 
-scoped[LO.FirstOrder] postfix:max "ᴺ" => Theory.doubleNegation
-
 abbrev Sequent.doubleNegation (Γ : List (Semiformula L ξ n)) : List (Semiformulaᵢ L ξ n) := Γ.map (·ᴺ)
 
 scoped[LO.FirstOrder] postfix:max "ᴺ" => Sequent.doubleNegation
 
+def Theory.ToTheoryᵢ (T : Theory L) (Λ : Hilbertᵢ L) : Theoryᵢ L Λ where
+  theory := Semiformula.doubleNegation '' T
+
+@[simp] lemma Theory.ToTheoryᵢ_theory_def (T : Theory L) (Λ : Hilbertᵢ L) :
+    (T.ToTheoryᵢ Λ).theory = Semiformula.doubleNegation '' T := rfl
+
 namespace Derivation
 
-variable {L : Language} [L.DecidableEq] {T : Theory L}
+variable {L : Language} [L.DecidableEq] {T : Theory L} {Λ : Hilbertᵢ L}
 
 open Rewriting LO.Entailment Entailment.FiniteContext HilbertProofᵢ
 
 noncomputable
-def negDoubleNegation : (φ : SyntacticFormula L) → 𝗠𝗶𝗻¹ ⊢! ∼φᴺ ⭤ (∼φ)ᴺ
+def negDoubleNegation : (φ : SyntacticFormula L) → Λ ⊢! ∼φᴺ ⭤ (∼φ)ᴺ
   | .rel r v  => Entailment.tneIff (φ := Semiformulaᵢ.rel r v)
   | .nrel r v => Entailment.E_Id (φ := ∼∼(Semiformulaᵢ.rel r v))
   | ⊤         => Entailment.ENNOO
   | ⊥         => Entailment.E_Id (φ := ∼⊥)
   | φ ⋏ ψ     =>
-    have ihφ : 𝗠𝗶𝗻¹ ⊢! ∼φᴺ ⭤ (∼φ)ᴺ := negDoubleNegation φ
-    have ihψ : 𝗠𝗶𝗻¹ ⊢! ∼ψᴺ ⭤ (∼ψ)ᴺ := negDoubleNegation ψ
-    have : 𝗠𝗶𝗻¹ ⊢! φᴺ ⋏ ψᴺ ⭤ ∼(∼φ)ᴺ ⋏ ∼(∼ψ)ᴺ :=
+    have ihφ : Λ ⊢! ∼φᴺ ⭤ (∼φ)ᴺ := negDoubleNegation φ
+    have ihψ : Λ ⊢! ∼ψᴺ ⭤ (∼ψ)ᴺ := negDoubleNegation ψ
+    have : Λ ⊢! φᴺ ⋏ ψᴺ ⭤ ∼(∼φ)ᴺ ⋏ ∼(∼ψ)ᴺ :=
       Entailment.EKK_of_E_of_E (iffnegOfNegIff (by simp) ihφ) (iffnegOfNegIff (by simp) ihψ)
     Entailment.ENN_of_E this
   | φ ⋎ ψ     =>
-    have ihφ : 𝗠𝗶𝗻¹ ⊢! ∼φᴺ ⭤ (∼φ)ᴺ := negDoubleNegation φ
-    have ihψ : 𝗠𝗶𝗻¹ ⊢! ∼ψᴺ ⭤ (∼ψ)ᴺ := negDoubleNegation ψ
-    have : 𝗠𝗶𝗻¹ ⊢! ∼φᴺ ⋏ ∼ψᴺ ⭤ (∼φ)ᴺ ⋏ (∼ψ)ᴺ := Entailment.EKK_of_E_of_E ihφ ihψ
-    have : 𝗠𝗶𝗻¹ ⊢! ∼∼(∼φᴺ ⋏ ∼ψᴺ) ⭤ (∼φ)ᴺ ⋏ (∼ψ)ᴺ := Entailment.E_trans (DN_of_isNegative (by simp)) this
+    have ihφ : Λ ⊢! ∼φᴺ ⭤ (∼φ)ᴺ := negDoubleNegation φ
+    have ihψ : Λ ⊢! ∼ψᴺ ⭤ (∼ψ)ᴺ := negDoubleNegation ψ
+    have : Λ ⊢! ∼φᴺ ⋏ ∼ψᴺ ⭤ (∼φ)ᴺ ⋏ (∼ψ)ᴺ := Entailment.EKK_of_E_of_E ihφ ihψ
+    have : Λ ⊢! ∼∼(∼φᴺ ⋏ ∼ψᴺ) ⭤ (∼φ)ᴺ ⋏ (∼ψ)ᴺ := Entailment.E_trans (DN_of_isNegative (by simp)) this
     this
   | ∀' φ      =>
-    have ihφ : 𝗠𝗶𝗻¹ ⊢! ∼(free φ)ᴺ ⭤ (∼(free φ))ᴺ := negDoubleNegation (free φ)
-    have : 𝗠𝗶𝗻¹ ⊢! (free φ)ᴺ ⭤ (∼(∼(free φ))ᴺ) := iffnegOfNegIff (by simp) ihφ
-    have : 𝗠𝗶𝗻¹ ⊢! ∀' φᴺ ⭤ ∀' ∼(∼φ)ᴺ :=
+    have ihφ : Λ ⊢! ∼(free φ)ᴺ ⭤ (∼(free φ))ᴺ := negDoubleNegation (free φ)
+    have : Λ ⊢! (free φ)ᴺ ⭤ (∼(∼(free φ))ᴺ) := iffnegOfNegIff (by simp) ihφ
+    have : Λ ⊢! ∀' φᴺ ⭤ ∀' ∼(∼φ)ᴺ :=
       allIffAllOfIff <| Entailment.cast (by simp [Semiformula.rew_doubleNegation]) this
     Entailment.ENN_of_E this
   | ∃' φ      =>
-    have ihφ : 𝗠𝗶𝗻¹ ⊢! ∼(free φ)ᴺ ⭤ (∼(free φ))ᴺ := negDoubleNegation (free φ)
-    have : 𝗠𝗶𝗻¹ ⊢! ∀' ∼φᴺ ⭤ ∀' (∼φ)ᴺ :=
+    have ihφ : Λ ⊢! ∼(free φ)ᴺ ⭤ (∼(free φ))ᴺ := negDoubleNegation (free φ)
+    have : Λ ⊢! ∀' ∼φᴺ ⭤ ∀' (∼φ)ᴺ :=
       allIffAllOfIff <| Entailment.cast (by simp [Semiformula.rew_doubleNegation]) ihφ
-    have : 𝗠𝗶𝗻¹ ⊢! ∼∼(∀' ∼φᴺ) ⭤ ∀' (∼φ)ᴺ := Entailment.E_trans (DN_of_isNegative (by simp)) this
+    have : Λ ⊢! ∼∼(∀' ∼φᴺ) ⭤ ∀' (∼φ)ᴺ := Entailment.E_trans (DN_of_isNegative (by simp)) this
     this
   termination_by φ => φ.complexity
+
+lemma neg_doubleNegation (φ : SyntacticFormula L) : Λ ⊢ ∼φᴺ ⭤ (∼φ)ᴺ := ⟨negDoubleNegation φ⟩
+
+lemma neg_doubleNegation' (φ : SyntacticFormula L) : Λ ⊢ ∼(∼φ)ᴺ ⭤ φᴺ := by simpa using neg_doubleNegation (∼φ)
+
+open FiniteContext
+
+lemma imply_doubleNegation (φ ψ : SyntacticFormula L) : Λ ⊢ (φᴺ ➝ ψᴺ) ⭤ (φ ➝ ψ)ᴺ := by
+  suffices Λ ⊢ (φᴺ ➝ ψᴺ) ⭤ ∼(∼(∼φ)ᴺ ⋏ ∼ψᴺ) by simpa [Semiformula.doubleNegation_imply]
+  have hφ₀ : Λ ⊢ ∼(∼φ)ᴺ ⭤ φᴺ := by simpa using neg_doubleNegation (∼φ)
+  have hψ : Λ ⊢ ∼∼ψᴺ ⭤ ψᴺ := ⟨DN_of_isNegative (by simp)⟩
+  apply Entailment.E!_intro
+  · apply FiniteContext.deduct'!
+    apply FiniteContext.deduct!
+    let Γ := [∼(∼φ)ᴺ ⋏ ∼ψᴺ, φᴺ ➝ ψᴺ]
+    have : Γ ⊢[Λ] φᴺ := of'! (K!_left hφ₀) ⨀ (K!_left by_axm₀!)
+    have : Γ ⊢[Λ] ψᴺ := by_axm₁! ⨀ this
+    exact K!_right by_axm₀! ⨀ this
+  · apply FiniteContext.deduct'!
+    apply FiniteContext.deduct!
+    refine of'! (K!_left hψ) ⨀ ?_
+    apply FiniteContext.deduct!
+    let Γ := [∼ψᴺ, φᴺ, ∼(∼(∼φ)ᴺ ⋏ ∼ψᴺ)]
+    have : Γ ⊢[Λ] ∼(∼φ)ᴺ := of'! (Γ := Γ) (K!_right hφ₀) ⨀ by_axm₁!
+    exact by_axm₂! ⨀ (K!_intro this by_axm₀!)
 
 open Entailment
 
 noncomputable
-def gödelGentzen {Γ : Sequent L} : ⊢ᵀ Γ → (∼Γ)ᴺ ⊢[𝗠𝗶𝗻¹]! ⊥
+def gödelGentzen {Γ : Sequent L} : ⊢ᵀ Γ → (∼Γ)ᴺ ⊢[Λ]! ⊥
   | axL Γ r v            => nthAxm 1 ⨀ nthAxm 0
   | verum Γ              => nthAxm 0
   | @and _ _ Γ φ ψ dφ dψ =>
-    have ihφ : ((∼φ)ᴺ :: (∼Γ)ᴺ) ⊢[𝗠𝗶𝗻¹]! ⊥ := gödelGentzen dφ
-    have ihψ : ((∼ψ)ᴺ :: (∼Γ)ᴺ) ⊢[𝗠𝗶𝗻¹]! ⊥ := gödelGentzen dψ
-    have : (∼Γ)ᴺ ⊢[𝗠𝗶𝗻¹]! ∼(∼φ)ᴺ ⋏ ∼(∼ψ)ᴺ := Entailment.K_intro (deduct ihφ) (deduct ihψ)
+    have ihφ : ((∼φ)ᴺ :: (∼Γ)ᴺ) ⊢[Λ]! ⊥ := gödelGentzen dφ
+    have ihψ : ((∼ψ)ᴺ :: (∼Γ)ᴺ) ⊢[Λ]! ⊥ := gödelGentzen dψ
+    have : (∼Γ)ᴺ ⊢[Λ]! ∼(∼φ)ᴺ ⋏ ∼(∼ψ)ᴺ := Entailment.K_intro (deduct ihφ) (deduct ihψ)
     deductInv (Entailment.dni' this)
   | @or _ _ Γ φ ψ d      =>
-    have : (∼Γ)ᴺ ⊢[𝗠𝗶𝗻¹]! (∼ψ)ᴺ ➝ (∼φ)ᴺ ➝ ⊥ := deduct <| deduct  <| gödelGentzen d
-    have : ((∼φ)ᴺ ⋏ (∼ψ)ᴺ :: (∼Γ)ᴺ) ⊢[𝗠𝗶𝗻¹]! ⊥ :=
+    have : (∼Γ)ᴺ ⊢[Λ]! (∼ψ)ᴺ ➝ (∼φ)ᴺ ➝ ⊥ := deduct <| deduct  <| gödelGentzen d
+    have : ((∼φ)ᴺ ⋏ (∼ψ)ᴺ :: (∼Γ)ᴺ) ⊢[Λ]! ⊥ :=
       Entailment.FiniteContext.weakening (by simp) this ⨀ (Entailment.K_right (nthAxm 0)) ⨀ (Entailment.K_left (nthAxm 0))
     this
   | @all _ _ Γ φ d       =>
     have eΓ : (∼Γ⁺)ᴺ = ((∼Γ)ᴺ)⁺ := by
       simp [Sequent.doubleNegation, Rewriting.shifts, Sequent.neg_def, Semiformula.rew_doubleNegation]
-    have : ((∼Γ)ᴺ)⁺ ⊢[𝗠𝗶𝗻¹]! free (∼(∼φ)ᴺ) :=
+    have : ((∼Γ)ᴺ)⁺ ⊢[Λ]! free (∼(∼φ)ᴺ) :=
       FiniteContext.cast (deduct (gödelGentzen d)) eΓ (by simp [Semiformula.rew_doubleNegation]; rfl)
     deductInv <| dni' <| geNOverFiniteContext this
   | @ex _ _ Γ φ t d      =>
-    have ih : (∼Γ)ᴺ ⊢[𝗠𝗶𝗻¹]! ∼((∼φ)ᴺ/[t]) :=
+    have ih : (∼Γ)ᴺ ⊢[Λ]! ∼((∼φ)ᴺ/[t]) :=
       Entailment.cast (by simp [Semiformula.rew_doubleNegation]; rfl) <| deduct (gödelGentzen d)
-    have : ((∀' (∼φ)ᴺ) :: (∼Γ)ᴺ) ⊢[𝗠𝗶𝗻¹]! (∼φ)ᴺ/[t] := specializeOverContext (nthAxm 0) t
+    have : ((∀' (∼φ)ᴺ) :: (∼Γ)ᴺ) ⊢[Λ]! (∼φ)ᴺ/[t] := specializeOverContext (nthAxm 0) t
     (FiniteContext.weakening (by simp) ih) ⨀ this
   | @cut _ _ Γ φ dp dn   =>
-    have ihp : ((∼φ)ᴺ :: (∼Γ)ᴺ) ⊢[𝗠𝗶𝗻¹]! ⊥ := gödelGentzen dp
-    have ihn : (φᴺ :: (∼Γ)ᴺ) ⊢[𝗠𝗶𝗻¹]! ⊥ := cast (by simp) (gödelGentzen dn)
-    have b₁ : (∼Γ)ᴺ ⊢[𝗠𝗶𝗻¹]! ∼∼φᴺ := Entailment.C_trans (of <| Entailment.K_left (negDoubleNegation φ)) (deduct ihp)
-    have b₂ : (∼Γ)ᴺ ⊢[𝗠𝗶𝗻¹]! ∼φᴺ := deduct ihn
+    have ihp : ((∼φ)ᴺ :: (∼Γ)ᴺ) ⊢[Λ]! ⊥ := gödelGentzen dp
+    have ihn : (φᴺ :: (∼Γ)ᴺ) ⊢[Λ]! ⊥ := cast (by simp) (gödelGentzen dn)
+    have b₁ : (∼Γ)ᴺ ⊢[Λ]! ∼∼φᴺ := Entailment.C_trans (of <| Entailment.K_left (negDoubleNegation φ)) (deduct ihp)
+    have b₂ : (∼Γ)ᴺ ⊢[Λ]! ∼φᴺ := deduct ihn
     b₁ ⨀ b₂
   | @wk _ _ Γ Δ d h      => FiniteContext.weakening (by simpa using List.map_subset _ h) (gödelGentzen d)
 
 end Derivation
 
-open Classical Entailment
+open Classical LO.Entailment
 
-lemma neg_doubleNegation (φ : SyntacticFormula L) : 𝗠𝗶𝗻¹ ⊢ ∼φᴺ ⭤ (∼φ)ᴺ := ⟨Derivation.negDoubleNegation φ⟩
-
-lemma GödelGentzen {φ} : (∅ : Theory L) ⊢ φ → (∅ : Theoryᵢ L 𝗠𝗶𝗻¹) ⊢ φᴺ := by
+/-- Gödel-Gentzen translation of classical first-order logic to intiotionistic first-order logic. -/
+theorem gödel_gentzen {T : Theory L} {φ} : T ⊢ φ → T.ToTheoryᵢ Λ ⊢ φᴺ := by
   intro h
-  let ψ : SyntacticFormula L := ↑φ
-  have h : (∅ : SyntacticFormulas L) ⊢ ↑φ := Entailment.wk! (by simp) h
-  have h₁ : 𝗠𝗶𝗻¹ ⊢ ∼(∼ψ)ᴺ := by
+  let ⟨⟨s, hs⟩, b⟩ := Theory.compact' h
+  have h : (∅ : SyntacticFormulas L) ⊢ ↑s.conj ➝ ↑φ := by simpa using provable_def.mp b
+  let ψ : SyntacticFormula L := ↑s.conj ➝ ↑φ
+  have h₁ : Λ ⊢ ∼(∼ψ)ᴺ := by
     simpa using Entailment.FiniteContext.provable_iff.mp ⟨Derivation.gödelGentzen h.get⟩
-  have h₂ : 𝗠𝗶𝗻¹ ⊢ ∼(∼ψ)ᴺ ⭤ ψᴺ := by simpa using neg_doubleNegation (∼ψ)
-  have : 𝗠𝗶𝗻¹ ⊢ Rewriting.emb φᴺ := by simpa [ψ, Semiformula.emb_doubleNegation] using Entailment.K!_left h₂ ⨀ h₁
-  exact Theoryᵢ.provable_def.mpr <| Entailment.Context.of! this
+  have h₂ : Λ ⊢ ∼(∼ψ)ᴺ ⭤ ψᴺ := by simpa using Derivation.neg_doubleNegation (∼ψ)
+  have : Λ ⊢ ψᴺ := K!_left h₂ ⨀ h₁
+  have H : Λ ⊢ (↑s.conj : SyntacticFormula L)ᴺ ➝ ↑φᴺ :=
+    by simpa [Semiformula.emb_doubleNegation] using (K!_right (Derivation.imply_doubleNegation _ _)) ⨀ this
+  let U : Set (SyntacticFormulaᵢ L) := (Rewriting.emb '' (T.ToTheoryᵢ Λ).theory)
+  suffices
+      U *⊢[Λ] ⋀ s.toList.map fun φ : Sentence L ↦ (↑φ : SyntacticFormula L)ᴺ by
+    apply Theoryᵢ.provable_def.mpr
+    apply Context.of! H ⨀ ?_
+    simpa [Finset.conj, List.map_conj₂, Function.comp_def]
+  apply LO.Entailment.Conj₂!_intro
+  have : ∀ ψ ∈ s, U *⊢[Λ] ↑ψᴺ := by
+    intro ψ hψ
+    exact Context.by_axm (by simpa [U] using ⟨ψ, hs hψ, rfl⟩)
+  simpa [←Semiformula.emb_doubleNegation] using this
 
 end LO.FirstOrder
